theories/core/utp_poly_expr.thy
@@ -1,0 +1,66 @@
+(******************************************************************************)
+(* Project: Unifying Theories of Programming in HOL                           *)
+(* File: utp_poly_expr.thy                                                    *)
+(* Author: Simon Foster and Frank Zeyda, University of York (UK)              *)
+(******************************************************************************)
+
+header {* Somewhat Polymorphic Expressions *}
+
+theory utp_poly_expr
+imports utp_expr
+begin
+
+type_synonym 'a PEXPRESSION = "'a UTYPE \<Rightarrow> 'a WF_EXPRESSION"
+
+definition WF_PEXPRESSION :: "'VALUE PEXPRESSION set" where
+"WF_PEXPRESSION = {f. \<forall> t. f t :\<^sub>e t}"
+
+typedef 'VALUE WF_PEXPRESSION = "WF_PEXPRESSION :: 'VALUE PEXPRESSION set"
+  apply (simp add:WF_PEXPRESSION_def)
+  apply (rule_tac x="(\<lambda> t. DefaultE t)" in exI)
+  apply (auto intro:typing)
+done
+
+declare Rep_WF_PEXPRESSION [simp]
+declare Rep_WF_PEXPRESSION_inverse [simp]
+declare Abs_WF_PEXPRESSION_inverse [simp]
+
+lemma Rep_WF_PEXPRESSION_intro [intro]:
+  "Rep_WF_PEXPRESSION x = Rep_WF_PEXPRESSION y \<Longrightarrow> x = y"
+  by (simp add:Rep_WF_PEXPRESSION_inject)
+
+lemma Rep_WF_PEXPRESSION_elim [elim]:
+  "\<lbrakk> x = y; Rep_WF_PEXPRESSION x = Rep_WF_PEXPRESSION y \<Longrightarrow> P \<rbrakk> \<Longrightarrow> P"
+  by (auto)
+
+setup_lifting type_definition_WF_PEXPRESSION
+
+notation Rep_WF_PEXPRESSION ("\<langle>_\<rangle>\<^sub>~")
+
+lemma Rep_WF_EXPRESSION_typed [typing]:
+  "\<langle>e\<rangle>\<^sub>~ t :\<^sub>e t"
+  apply (insert Rep_WF_PEXPRESSION[of e])
+  apply (auto simp add:WF_PEXPRESSION_def)
+done
+
+definition CoercePE :: "'a WF_PEXPRESSION \<Rightarrow> 'a UTYPE \<Rightarrow> 'a WF_EXPRESSION" where
+"CoercePE e t = \<langle>e\<rangle>\<^sub>~ t"
+
+subsection {* List Expressions *}
+
+lift_definition NilPE :: "'a::{BOT_SORT, LIST_SORT} WF_PEXPRESSION" 
+is "\<lambda> a. if (isListType a \<and> ListParam a \<in> ListPerm) 
+         then NilE (ListParam a) else BotE a"
+  by (force intro:typing simp add:WF_PEXPRESSION_def)
+
+lift_definition ConsPE :: 
+  "'a::{BOT_SORT, LIST_SORT} WF_PEXPRESSION \<Rightarrow> 'a WF_PEXPRESSION \<Rightarrow> 'a WF_PEXPRESSION" 
+is "\<lambda> x xs a. if (isListType a \<and> ListParam a \<in> ListPerm \<and> \<D> (x (ListParam a)) \<and> \<D> (xs a))
+              then ConsE (ListParam a) (x (ListParam a)) (xs a) else BotE a"
+  by (force intro:typing simp add:WF_PEXPRESSION_def)
+
+(* Convert to an fully disambiguated polymorphic expression to a basic expression *)
+definition PExprE :: "'a WF_PEXPRESSION \<Rightarrow> 'a WF_EXPRESSION" where
+"PExprE e = \<langle>e\<rangle>\<^sub>~ (THE t. \<D> (\<langle>e\<rangle>\<^sub>~ t))"
+
+end
